theories/examples/template_adequacy_ocpl.v
@@ -5,7 +5,7 @@ From iris.program_logic Require Import adequacy.
 From cap_machine Require Import
      stdpp_extra iris_extra
      rules logrel fundamental.
-From cap_machine.examples Require Import addr_reg_sample malloc macros_new.
+From cap_machine.examples Require Import addr_reg_sample malloc assert macros_new.
 From cap_machine.examples Require Export mkregion_helpers disjoint_regions_tactics.
 From cap_machine.examples Require Import template_adequacy.
 
@@ -29,26 +29,22 @@ Record ocpl_library `{MachineParameters} := MkOcplLibrary {
   malloc_mem_size :
     (malloc_mem_start <= malloc_end)%a;
 
-  (* assertion fail library *)
-  fail_start : Addr;
-  fail_end : Addr;
+  (* assert library *)
+  assert_start : Addr;
+  assert_cap : Addr;
+  assert_flag : Addr;
+  assert_end : Addr;
 
-  fail_size :
-    (fail_start
-     + (length assert_fail_instrs (* code of the subroutine *)
-        + 1 (* pointer to the flag *))
-    )%a
-    = Some fail_end;
-
-  fail_flag : Addr;
-  fail_flag_next : Addr;
-  fail_flag_size :
-    (fail_flag + 1)%a = Some fail_flag_next;
+  assert_code_size :
+    (assert_start + length assert_subroutine_instrs)%a = Some assert_cap;
+  assert_cap_size :
+    (assert_cap + 1)%a = Some assert_flag;
+  assert_flag_size :
+    (assert_flag + 1)%a = Some assert_end;
 
   (* disjointness of the two libraries *)
-  libs_disjoint :     ## [
-      [fail_flag];
-      region_addrs fail_start fail_end;
+  libs_disjoint : ## [
+      region_addrs assert_start assert_end;
       region_addrs malloc_mem_start malloc_end;
       [malloc_memptr];
       region_addrs malloc_start malloc_memptr
@@ -69,28 +65,29 @@ Definition lib_entry_malloc `{MachineParameters} (layout : ocpl_library) : lib_e
      lib_entrypoint := malloc_start layout;
      lib_full_content := malloc_library_content layout|}.
 
-(* FAIL library entry *)
-Definition fail_library_content `{MachineParameters} (layout : ocpl_library) : gmap Addr Word :=
-  (* code for the failure subroutine *)
-  (* tail contains pointer to the "failure" flag, set to 1 by the routine *)
-  mkregion (fail_start layout) (fail_end layout) (assert_fail_instrs ++ [WCap RW (fail_flag layout) (fail_flag_next layout) (fail_flag layout)])
-  ∪ list_to_map [((fail_flag layout), WInt 0%Z)] (* failure flag, initially set to 0 *).
+(* assert library entry *)
+Definition assert_library_content `{MachineParameters} (layout : ocpl_library) : gmap Addr Word :=
+  (* code for the assert subroutine, followed by a capability to the assert flag
+     and the flag itself, initialized to 0. *)
+  mkregion (assert_start layout) (assert_cap layout) assert_subroutine_instrs
+  ∪ list_to_map [(assert_cap layout, WCap RW (assert_flag layout) (assert_end layout) (assert_flag layout))]
+  ∪ list_to_map [(assert_flag layout, WInt 0)] (* assert flag *).
 
-Definition lib_entry_fail `{MachineParameters} (layout : ocpl_library) : lib_entry :=
-  {| lib_start := fail_start layout;
-     lib_end := fail_end layout;
-     lib_entrypoint := fail_start layout;
-     lib_full_content := fail_library_content layout |}.
+Definition lib_entry_assert `{MachineParameters} (layout : ocpl_library) : lib_entry :=
+  {| lib_start := assert_start layout;
+     lib_end := assert_end layout;
+     lib_entrypoint := assert_start layout;
+     lib_full_content := assert_library_content layout |}.
 
 (* full library *)
 Definition library `{MachineParameters} (layout : ocpl_library) : lib :=
-  {| priv_libs := [lib_entry_fail layout] ;
+  {| priv_libs := [lib_entry_assert layout] ;
      pub_libs := [lib_entry_malloc layout] |}.
 
 Definition OK_invariant `{MachineParameters} (layout : ocpl_library) (m : gmap Addr Word) : Prop :=
-  ∀ w, m !! (fail_flag layout) = Some w → w = WInt 0%Z.
+  ∀ w, m !! (assert_flag layout) = Some w → w = WInt 0%Z.
 
-Definition OK_dom `{MachineParameters} (layout : ocpl_library) : gset Addr := {[ fail_flag layout ]}.
+Definition OK_dom `{MachineParameters} (layout : ocpl_library) : gset Addr := {[ assert_flag layout ]}.
 
 Program Definition OK_dom_correct `{MachineParameters} (layout : ocpl_library) :
   ∀ m m',
@@ -98,13 +95,13 @@ Program Definition OK_dom_correct `{MachineParameters} (layout : ocpl_library) :
     OK_invariant layout m ↔ OK_invariant layout m'.
 Proof.
   intros m m' Hdom.
-  destruct Hdom with (fail_flag layout) as [w [Hw1 Hw2] ]. rewrite /OK_dom. set_solver.
+  destruct Hdom with (assert_flag layout) as [w [Hw1 Hw2] ]. rewrite /OK_dom. set_solver.
   split;intros HOK;intros w' Hw';simplify_eq;apply HOK;auto.
 Defined.
 
 Definition flag_inv `{MachineParameters} (layout : ocpl_library) : memory_inv :=
   {| minv := OK_invariant layout;
-     minv_dom := {[ fail_flag layout ]} ;
+     minv_dom := {[ assert_flag layout ]} ;
      minv_dom_correct := OK_dom_correct layout |}.
 
 Lemma flag_inv_is_initial_memory `{MachineParameters} (layout : ocpl_library) trusted_prog adv_prog trusted_table adv_table m :
@@ -114,17 +111,17 @@ Proof.
   intros Hinit. intros a Hin.
   destruct Hinit as (?&?&Hlibs&?&?&?&Hlibdisj).
   cbn in Hlibs. rewrite map_union_empty in Hlibs.
-  assert ((fail_library_content layout) ⊆ m) as Hfail.
+  assert ((assert_library_content layout) ⊆ m) as Hassert.
   { etrans;[|eauto]. apply map_union_subseteq_r. cbn in Hlibdisj.
     rewrite !map_union_empty in Hlibdisj. auto. }
-  rewrite /fail_library_content in Hfail.
-  assert (list_to_map [(fail_flag layout, WInt 0)] ⊆ m) as Hfail_flag.
-  { etrans;[|eauto]. apply map_union_subseteq_r. disjoint_map_to_list.
-    pose proof (libs_disjoint layout) as Hdisjoint.
-    rewrite !disjoint_list_cons in Hdisjoint |- *. intros (?&?&?&?&?&?).
-    set_solver. }
-  simpl in Hfail_flag.
-  eapply (lookup_weaken _ _ (fail_flag layout) (WInt 0)) in Hfail_flag.
+  pose proof (assert_code_size layout). pose proof (assert_cap_size layout).
+  pose proof (assert_flag_size layout).
+  assert (list_to_map [(assert_flag layout, WInt 0)] ⊆ m) as Hassert_flag.
+  { etrans;[|eauto]. eapply map_union_subseteq_r_alt. 2: done.
+    pose proof (libs_disjoint layout) as Hdisjoint. disjoint_map_to_list.
+    apply elem_of_disjoint. intro. rewrite elem_of_app !elem_of_region_addrs !elem_of_list_singleton.
+    intros [ [? ?]|?] ->; solve_addr. }
+  eapply (lookup_weaken _ _ (assert_flag layout) (WInt 0)) in Hassert_flag.
     by simplify_eq. by simplify_map_eq.
 Qed.
 
@@ -132,49 +129,21 @@ Lemma flag_inv_sub `{MachineParameters} (layout : ocpl_library) :
   minv_dom (flag_inv layout) ⊆ dom (gset Addr) (lib_region (priv_libs (library layout))).
 Proof.
   cbn. rewrite map_union_empty.
-  intros Hinit. rewrite /fail_library_content.
-  rewrite /= dom_union_L dom_insert_L dom_empty_L.
-  rewrite union_empty_r. apply union_subseteq_r.
+  intros ? Hinit. rewrite elem_of_singleton in Hinit |- * => ->.
+  rewrite /assert_library_content.
+  pose proof (assert_code_size layout). pose proof (assert_cap_size layout).
+  pose proof (assert_flag_size layout).
+  rewrite /= dom_union_L. apply elem_of_union_r.
+  rewrite dom_insert_L. set_solver.
 Qed.
-
-(* TODO: move to iris extra *)
-Lemma big_sepM_to_big_sepL2 (PROP : bi) (A B : Type) `{EqDecision A} `{Countable A}
-      (φ: A -> B -> PROP) (l1: list A) (l2: list B):
-      NoDup l1 -> length l1 = length l2 →
-      ⊢ (([∗ map] y1↦y2 ∈ list_to_map (zip l1 l2), φ y1 y2) -∗
-         ([∗ list] y1;y2 ∈ l1;l2, φ y1 y2))%I.
-Proof.
-  revert l2. iInduction (l1) as [|x l1] "IH"; iIntros (l2 Hnd Hlen) "H".
-  - iSimpl. destruct l2;inversion Hlen. done.
-  - destruct l2;inversion Hlen. simpl.
-    inversion Hnd. subst.
-    iDestruct (big_sepM_insert with "H") as "[A B]".
-    + eapply not_elem_of_list_to_map.
-      rewrite fst_zip; auto. lia.
-    + iFrame. iApply ("IH" $! l2 H4 H1 with "B"); auto.
-Qed.
-Lemma map_filter_id :
-  ∀ (K : Type) (M : Type → Type) (H : FMap M) (H0 : ∀ A : Type, Lookup K A (M A)) (H1 : ∀ A : Type, Empty (M A)) (H2 : ∀ A : Type, PartialAlter K A (M A))
-    (H3 : OMap M) (H4 : Merge M) (H5 : ∀ A : Type, FinMapToList K A (M A)) (EqDecision0 : EqDecision K),
-    FinMap K M
-    → ∀ (A : Type) (P : K * A → Prop) (H7 : ∀ x : K * A, Decision (P x)) (m : M A),
-      (∀ i x, m !! i = Some x → P (i, x)) → filter P m = m.
-Proof.
-  intros. apply map_eq.
-  intros i. destruct (m !! i) eqn:Hsome.
-  - apply map_filter_lookup_Some_2;auto.
-  - apply map_filter_lookup_None_2;auto.
-Qed.
-
-
 
 Definition assertInv `{memG Σ, regG Σ, MachineParameters} (layout : ocpl_library) :=
-  [[ fail_start layout, fail_end layout]]↦ₐ[[ assert_fail_instrs ++ [WCap RW (fail_flag layout) (fail_flag_next layout) (fail_flag layout)] ]]%I.
+  assert_inv (assert_start layout) (assert_flag layout) (assert_end layout).
 Definition mallocInv `{memG Σ, regG Σ, MachineParameters} (layout : ocpl_library) :=
   malloc_inv (malloc_start layout) (malloc_end layout).
 
 Definition mallocN : namespace := nroot .@ "pub" .@ "malloc".
-Definition failflagN : namespace := nroot .@ "priv" .@ "flag".
+Definition assertN : namespace := nroot .@ "priv" .@ "assert".
 
 Theorem ocpl_template_adequacy `{MachineParameters} (Σ : gFunctors)
     (layout: ocpl_library)
@@ -191,7 +160,7 @@ Theorem ocpl_template_adequacy `{MachineParameters} (Σ : gFunctors)
       dom (gset RegName) rmap = all_registers_s ∖ {[ PC; r_adv ]} →
       ⊢ inv invN (minv_sep (flag_inv layout))
         ∗ na_inv logrel_nais mallocN (mallocInv layout)
-        ∗ na_inv logrel_nais failflagN (assertInv layout)
+        ∗ na_inv logrel_nais assertN (assertInv layout)
         ∗ na_own logrel_nais ⊤
         ∗ PC ↦ᵣ WCap RWX (prog_lower_bound P_tbl) (prog_end P) (prog_start P)
         ∗ r_adv ↦ᵣ WCap RWX (prog_lower_bound Adv_tbl) (prog_end Adv) (prog_start Adv)
@@ -220,7 +189,7 @@ Proof.
   intros. cbn.
   rewrite !map_union_empty.
   iIntros "(#Hflag & Hown & HPC & Hr_adv & Hrmap & Htbl & Htbl_r
-           & Hprog & Htbl_adv & Htbl_adv_r & Hprog_adv & Hmalloc & Hfail)".
+           & Hprog & Htbl_adv & Htbl_adv_r & Hprog_adv & Hmalloc & Hassert)".
 
   (* allocate malloc invariant *)
   iMod (na_inv_alloc logrel_nais ⊤ mallocN (mallocInv layout)
@@ -229,11 +198,11 @@ Proof.
     rewrite /malloc_library_content.
     iDestruct (big_sepM_union with "Hmalloc") as "[Hpubs Hinit]".
     { pose proof (libs_disjoint layout) as Hdisjoint.
-      rewrite !disjoint_list_cons in Hdisjoint |- *. intros (?&?&?&?&?&?).
+      rewrite !disjoint_list_cons in Hdisjoint |- *. intros (?&?&?&?&?).
       disjoint_map_to_list. set_solver. }
     iDestruct (big_sepM_union with "Hpubs") as "[Hpubs Hmid]".
     { pose proof (libs_disjoint layout) as Hdisjoint.
-      rewrite !disjoint_list_cons in Hdisjoint |- *. intros (?&?&?&?&?&?).
+      rewrite !disjoint_list_cons in Hdisjoint |- *. intros (?&?&?&?&?).
       disjoint_map_to_list. set_solver. }
     pose proof (malloc_code_size layout) as Hmalloc_size.
     pose proof (malloc_memptr_size layout) as Hmalloc_memptr_size.
@@ -250,29 +219,34 @@ Proof.
     rewrite region_addrs_length replicate_length /region_size. solve_addr +Hmalloc_mem_size. iFrame. }
 
   (* allocate the flag invariant *)
-  iMod (na_inv_alloc logrel_nais ⊤ failflagN (assertInv layout)
-          with "[Hfail]") as "#Hinv_fail".
-  { iNext. rewrite /assertInv /fail_library_content.
-    rewrite -insert_union_r.
-    pose proof (fail_flag_size layout) as Hfail_flag_size.
-    pose proof (fail_size layout) as Hfail_size.
-    rewrite map_union_empty map_filter_insert_not'.
+  iMod (na_inv_alloc logrel_nais ⊤ assertN (assertInv layout)
+          with "[Hassert]") as "#Hinv_assert".
+  { iNext. rewrite /assertInv /assert_inv /assert_library_content.
+    iExists (assert_cap layout).
+    pose proof (assert_code_size layout). pose proof (assert_cap_size layout).
+    pose proof (assert_flag_size layout).
+    rewrite map_filter_union.
+    2: { disjoint_map_to_list. apply elem_of_disjoint. intro.
+         rewrite elem_of_app elem_of_region_addrs !elem_of_list_singleton.
+         intros [ [? ?]|?]; solve_addr. }
+    iDestruct (big_sepM_union with "Hassert") as "[Hassert _]".
+    { eapply map_filter_disjoint. typeclasses eauto. disjoint_map_to_list.
+      apply elem_of_disjoint. intro.
+      rewrite elem_of_app elem_of_region_addrs !elem_of_list_singleton.
+      intros [ [? ?]|?]; solve_addr. }
     rewrite map_filter_id.
-    - by iApply mkregion_sepM_to_sepL2.
-    - intros i x Hx.
-      assert (i ∈ region_addrs (fail_start layout) (fail_end layout)) as Hin.
-      { eapply in_dom_mkregion. apply elem_of_gmap_dom. eauto. }
-      intros Hcontr%elem_of_singleton_1. subst.
-      pose proof (libs_disjoint layout) as Hdisjoint.
-      rewrite !disjoint_list_cons in Hdisjoint |- *. intros (?&?&?&?&?&?).
-      set_solver.
-    - simpl. intros Hcontr. apply Hcontr. apply elem_of_singleton. auto.
-    - intros y _. intros Hcontr. apply Hcontr. apply elem_of_singleton. auto.
-    - apply not_elem_of_dom.
-      intros Hdom%in_dom_mkregion.
-      pose proof (libs_disjoint layout) as Hdisjoint.
-      rewrite !disjoint_list_cons in Hdisjoint |- *. intros (?&?&?&?&?&?).
-      set_solver. }
+    2: { intros ? ? HH%elem_of_dom_2. rewrite !dom_union_L dom_mkregion_eq in HH.
+         2: solve_addr. apply elem_of_union in HH.
+         rewrite elem_of_singleton. destruct HH as [HH|HH].
+         rewrite -> elem_of_list_to_set, elem_of_region_addrs in HH; solve_addr.
+         rewrite -> dom_list_to_map_singleton, elem_of_list_to_set, elem_of_list_singleton in HH; solve_addr. }
+    iDestruct (big_sepM_union with "Hassert") as "[Hassert Hcap]".
+    { disjoint_map_to_list. apply elem_of_disjoint. intro.
+      rewrite elem_of_region_addrs !elem_of_list_singleton. solve_addr. }
+    iDestruct (mkregion_sepM_to_sepL2 with "Hassert") as "Hassert". solve_addr.
+    rewrite (_: assert_cap layout = assert_start layout ^+ length assert_subroutine_instrs)%a. 2: solve_addr.
+    iFrame "Hassert". iDestruct (big_sepM_insert with "Hcap") as "[Hcap _]". done.
+    iFrame "Hcap". iPureIntro. repeat split; solve_addr. }
 
   iApply Hspec;[..|iFrame "∗ #"];auto. solve_inG.
 Qed.
