theories/examples/assert.v
@@ -1,0 +1,119 @@
+From iris.algebra Require Import frac.
+From iris.proofmode Require Import tactics.
+From cap_machine Require Import logrel addr_reg_sample fundamental rules proofmode.
+
+(* Assert routine *)
+
+(* Maintains a flag storing whether an assert has failed. *)
+
+Section Assert.
+  Context {Σ:gFunctors} {memg:memG Σ} {regg:regG Σ}
+          {nainv: logrel_na_invs Σ}
+          `{MP: MachineParameters}.
+
+  (* assert (r4 == r5) *)
+  Definition assert_subroutine_instrs :=
+    encodeInstrsW [
+      Sub r_t4 r_t4 r_t5;
+      Mov r_t5 PC;
+      Lea r_t5 6;
+      Jnz r_t5 r_t4;
+      (* success case *)
+      Mov r_t4 0;
+      Mov r_t5 0;
+      Jmp r_t0; (* return *)
+      (* failure case *)
+      Lea r_t5 6; (* pointer to cap: *)
+      Load r_t5 r_t5;
+      Store r_t5 1;
+      Mov r_t4 0;
+      Mov r_t5 0;
+      Jmp r_t0 (* return *)
+    ].
+  (* followed in memory by:
+    cap: (RW, flag, end, flag)
+    flag: <0 or 1>
+    end:
+  *)
+
+  Definition assert_inv (b a_flag e : Addr) : iProp Σ :=
+    (∃ cap_addr,
+       codefrag b assert_subroutine_instrs ∗
+       ⌜(b + length assert_subroutine_instrs)%a = Some cap_addr⌝ ∗
+       ⌜(cap_addr + 1)%a = Some a_flag⌝ ∗
+       ⌜(a_flag + 1)%a = Some e⌝ ∗
+       cap_addr ↦ₐ WCap RW a_flag e a_flag).
+
+  Lemma assert_subroutine_spec b a_flag e cont n1 n2 flag N E φ :
+    ↑N ⊆ E →
+    (  na_inv logrel_nais N (assert_inv b a_flag e)
+     ∗ na_own logrel_nais E
+     ∗ PC ↦ᵣ WCap RX b e b
+     ∗ r_t0 ↦ᵣ cont
+     ∗ r_t4 ↦ᵣ WInt n1
+     ∗ r_t5 ↦ᵣ WInt n2
+     ∗ a_flag ↦ₐ WInt flag
+     ∗ ▷ (na_own logrel_nais E
+          ∗ PC ↦ᵣ updatePcPerm cont
+          ∗ r_t0 ↦ᵣ cont
+          ∗ r_t4 ↦ᵣ WInt 0
+          ∗ r_t5 ↦ᵣ WInt 0
+          ∗ a_flag ↦ₐ WInt (if (n1 =? n2)%Z then flag else 1%Z)
+          -∗ WP Seq (Instr Executable) {{ φ }})
+     ⊢ WP Seq (Instr Executable) {{ φ }})%I.
+  Proof.
+    iIntros (HNE) "(#Hinv & Hna & HPC & Hr0 & Hr1 & Hr2 & Hflag & Hφ)".
+    iMod (na_inv_acc with "Hinv Hna") as "(>Hassert & Hna & Hinv_close)"; auto.
+    iDestruct "Hassert" as (cap_addr) "(Hprog & %Hcap & %Hflag & %He & Hcap)".
+    rewrite /assert_subroutine_instrs. codefrag_facts "Hprog".
+    assert (SubBounds b e b (b ^+ length assert_subroutine_instrs)%a) by solve_addr.
+    do 3 iInstr "Hprog".
+    destruct (decide (n1 = n2)).
+    { (* n1 = n2 *)
+      subst n2. rewrite (_: n1 - n1 = 0)%Z; last lia.
+      iGo "Hprog".
+      iMod ("Hinv_close" with "[Hprog Hcap $Hna]") as "Hna".
+      { iExists _. iNext. iFrame. iPureIntro. repeat split; solve_addr. }
+      iApply "Hφ". iFrame. rewrite Z.eqb_refl //. }
+    { (* n1 ≠ n2 *)
+      iInstr "Hprog". { assert (n1 - n2 ≠ 0)%Z by lia. congruence. }
+      iInstr "Hprog". rewrite (_: (b ^+ 13)%a = cap_addr). 2: solve_addr.
+      iInstr "Hprog". solve_addr.
+      iInstr "Hprog". solve_addr.
+      iGo "Hprog".
+      iMod ("Hinv_close" with "[Hprog Hcap $Hna]") as "Hna".
+      { iExists _. iNext. iFrame. iPureIntro. repeat split; solve_addr. }
+      iApply "Hφ". iFrame. rewrite (_: (n1 =? n2)%Z = false) //.
+      by apply Z.eqb_neq. }
+  Qed.
+
+  Lemma assert_success_spec b a_flag e cont n1 n2 N E φ :
+    ↑N ⊆ E →
+    n1 = n2 →
+    (  na_inv logrel_nais N (assert_inv b a_flag e)
+     ∗ na_own logrel_nais E
+     ∗ PC ↦ᵣ WCap RX b e b
+     ∗ r_t0 ↦ᵣ cont
+     ∗ r_t4 ↦ᵣ WInt n1
+     ∗ r_t5 ↦ᵣ WInt n2
+     ∗ ▷ (na_own logrel_nais E
+          ∗ PC ↦ᵣ updatePcPerm cont
+          ∗ r_t0 ↦ᵣ cont
+          ∗ r_t4 ↦ᵣ WInt 0
+          ∗ r_t5 ↦ᵣ WInt 0
+          -∗ WP Seq (Instr Executable) {{ φ }})
+     ⊢ WP Seq (Instr Executable) {{ φ }})%I.
+  Proof.
+    iIntros (HNE Heq) "(#Hinv & Hna & HPC & Hr0 & Hr1 & Hr2 & Hφ)".
+    iMod (na_inv_acc with "Hinv Hna") as "(>Hassert & Hna & Hinv_close)"; auto.
+    iDestruct "Hassert" as (cap_addr) "(Hprog & %Hcap & %Hflag & %He & Hcap)".
+    rewrite /assert_subroutine_instrs. codefrag_facts "Hprog".
+    assert (SubBounds b e b (b ^+ length assert_subroutine_instrs)%a) by solve_addr.
+    do 3 iInstr "Hprog". rewrite (_: n1 - n2 = 0)%Z; last lia.
+    iGo "Hprog".
+    iMod ("Hinv_close" with "[Hprog Hcap $Hna]") as "Hna".
+    { iExists _. iNext. iFrame. iPureIntro. repeat split; solve_addr. }
+    iApply "Hφ". iFrame.
+  Qed.
+
+End Assert.
